Blocks.v
@@ -10,7 +10,7 @@ Section Blocks.
 Variable maxReg : nat.          (* max number of registers *)
 Definition PhysReg : predArgType := 'I_maxReg.
 
-Inductive VarKind : Set := Input | Temp | Output | InputOutput.
+Inductive VarKind : Set := Input | Temp | Output.
 
 Section EqVarKind.
 
@@ -18,11 +18,10 @@ Implicit Type s : VarKind.
 
 Fixpoint eqVarKind s1 s2 {struct s2} :=
   match s1, s2 with
-  | Input, Input             => true
-  | Temp, Temp               => true
-  | Output, Output           => true
-  | InputOutput, InputOutput => true
-  | _, _ => false
+  | Input, Input   => true
+  | Temp, Temp     => true
+  | Output, Output => true
+  | _, _           => false
   end.
 
 Lemma eqVarKindP : Equality.axiom eqVarKind.
@@ -123,5 +122,4 @@ Tactic Notation "VarKind_cases" tactic(first) ident(c) :=
   [ Case_aux c "VarKind_Input"
   | Case_aux c "VarKind_Temp"
   | Case_aux c "VarKind_Output"
-  | Case_aux c "VarKind_InputOutput"
   ].
